
@prefix : <http://set.win.tue.nl/ontology#> .
@prefix rdfs:	<http://www.w3.org/2000/01/rdf-schema#> . 
@prefix rdf:	<http://www.w3.org/1999/02/22-rdf-syntax-ns#> . 
@prefix owl:	<http://www.w3.org/2002/07/owl#> .
@base <http://set.win.tue.nl/ontology#> .

<http://set.win.tue.nl/ontology>
	rdf:type owl:Ontology .

:container
    rdf:type        rdfs:Class;
    rdfs:comment    "Something that can contain a structure (or another container), e.g., package, module, directory, file."@en.

:type
    rdf:type        rdfs:Class;
    rdfs:comment    "Something that variable can be a type of; can be a primitive or a structure."@en.

:structure
    rdf:type        rdfs:Class;
    rdfs:subClassOf :type;
    rdfs:subClassOf :container;
    rdfs:comment    "A complex/compound type, e.g., a class, record, struct, etc."@en.

:primitive
    rdf:type        rdfs:Class;
    rdfs:subClassOf :type;
    rdfs:comment    "A primitive type, e.g., int, boolean."@en.

:script
    rdf:type        rdfs:Class;
    rdfs:comment    "A collection of program statements."@en.

:operation
    rdf:type        rdfs:Class;
    rdfs:subClassOf :script;
    rdfs:comment    "A script that has a name/signature, i.e., a function, procedure, or method."@en.

:constructor
    rdf:type        rdfs:Class;
    rdfs:subClassOf :operation;
    rdfs:comment    "A special type of operation that instantiates a structure/initializes an object."@en.

:variable
    rdf:type        rdfs:Class;
    rdfs:comment    "Something that holds value(s), e.g., a variable or a field in a class."@en.


:typed
    rdf:type        rdf:Property;
    rdfs:domain     :variable;
    rdfs:range      :type;
    rdfs:comment    "A property that defines a variable's type."@en.

:specializes
    rdf:type        rdf:Property;
    rdfs:domain     :structure;
    rdfs:range      :structure;
    rdfs:comment    "A property that defines structure specialization, e.g., a structure is a subclass of another structure."@en.

:hasVariable
    rdf:type        rdf:Property;
    rdfs:domain     :structure;
    rdfs:range      :variable;
    rdfs:comment    "A property that defines the data part of a structure, e.g., attributes of a class."@en.

:hasScript
    rdf:type        rdf:Property;
    rdfs:domain     :structure;
    rdfs:range      :script;
    rdfs:comment    "A property that defines behaviors of a structure, e.g., methods in a class."@en.

:instantiates
    rdf:type        rdf:Property;
    rdfs:domain     :script;
    rdfs:range      :structure;
    rdfs:comment    "A property that shows that a script contains a call to a structure's constructor."@en.

:invokes
    rdf:type        rdf:Property;
    rdfs:domain     :script;
    rdfs:range      :operation;
    rdfs:comment    "A property that shows that a script contains a call to an operation."@en.

:hasReturnType
    rdf:type        rdf:Property;
    rdfs:domain     :operation;
    rdfs:range      :type;
    rdfs:comment    "A property that defines the return type of an operation."@en.

:hasParameterType
    rdf:type        rdf:Property;
    rdfs:domain     :operation;
    rdfs:range      :type;
    rdfs:comment    "A property that defines a parameter type that an operation accepts."@en.


:depends
    rdf:type        rdf:Property;
    rdfs:domain     :structure;
    rdfs:range      :structure;
    rdfs:comment    "A property that defines an operational dependency between classes; a simplification of the hasScript->invokes properties."@en.

:constructs
    rdf:type        rdf:Property;
    rdfs:domain     :structure;
    rdfs:range      :structure;
    rdfs:comment    "A property shows that a structure calls another structure's constructor; a simplification of the hasScript->instantiates properties."@en.

:holds
    rdf:type        rdf:Property;
    rdfs:domain     :structure;
    rdfs:range      :type;
    rdfs:comment    "A property that defines a has-a relationship between a structure and a type; a simplification of the hasVariable->typed properties."@en.

:depends
    rdf:type        rdf:Property;
    rdfs:domain     :structure;
    rdfs:range      :type;
    rdfs:comment    "A property that shows that a structure accepts a type as parameter to its operation(s); a simplification of the hasScript->hasParameterType properties."@en.

:returns
    rdf:type        rdf:Property;
    rdfs:domain     :structure;
    rdfs:range      :type;
    rdfs:comment    "A property that shows that a structure has operation(s) that returns a value with particular type; a simplification of the hasScript->returnType properties."@en.




:named
	rdf:type		rdf:Property;
	rdfs:domain		:structural_unit;
	rdfs:range		rdfs:Literal;
	rdfs:comment	"name of a structural unit"@en.

:kind
	rdf:type		rdf:Property;
	rdfs:domain		:structure;
	rdfs:range		rdfs:Literal;
	rdfs:comment	"The kind of a class, e.g., abstract, interface, enum."@en.

:design_pattern
	rdf:type		rdfs:Class;
	rdfs:type		rdfs:Class;
	rdfs:comment	"general design pattern"@en.

:role
	rdf:type		rdfs:Class;
	rdfs:type		rdfs:Class;
	rdfs:comment	"role in a design pattern"@en.

:part_of
	rdf:type		rdf:Property;
	rdfs:domain		:role;
	rdfs:range		:design_pattern;
	rdfs:comment 	"role is part of design pattern"@en.

:manifests
	rdf:type		rdf:Property;
	rdfs:domain		:structural_unit;
	rdfs:range		:role;
	rdfs:comment	"a structural unit manifests a role in a design pattern"@en.